src/Symbolic/SymbExamples.v
@@ -1,0 +1,229 @@
+From CoreErlang.FrameStack Require Import SubstSemantics SubstSemanticsLemmas.
+From CoreErlang.Interpreter Require Import StepFunctions Equivalences.
+From CoreErlang.Symbolic Require Import SymbTheorems SymbTactics.
+
+Import ListNotations.
+
+Definition fact_frameStack (e : Exp) : Exp :=
+  ELetRec
+    [(1, °ECase (˝VVar 1) [
+      ([PLit 0%Z], ˝ttrue, (˝VLit 1%Z));
+      ([PVar], ˝ttrue,
+        °ELet 1 (EApp (˝VFunId (1, 1))
+          [°ECall (˝VLit "erlang"%string) (˝VLit "-"%string) [˝VVar 0; ˝VLit 1%Z]])
+          (°ECall (˝VLit "erlang"%string) (˝VLit "*"%string) [˝VVar 1; ˝VVar 0])
+      )
+    ])]
+    (EApp (˝VFunId (0, 1)) [e])
+   (* Write the definition here *)
+.
+
+Theorem fact_eval_ex:
+  forall (z : Z), (0 <= z)%Z ->
+  exists (y : Z),
+  ⟨ [], (fact_frameStack (˝VLit z)) ⟩ -->* RValSeq [VLit y] /\ (z <= y /\ y >= 1)%Z.
+Proof.
+  solve_symbolically z.
+Qed.
+
+Definition tailrec_fact (e d : Exp) : Exp :=
+  ELetRec [
+    (2, °ECase (˝VVar 1) [
+        ([PLit (Integer 0%Z)], ˝ttrue, ˝VVar 2);
+        ([PVar], ˝ttrue,
+          (°EApp (˝VFunId (1, 2)) 
+            [°ECall (˝erlang) (˝VLit "-"%string) [˝VVar 0; ˝VLit 1%Z];
+             °ECall (˝erlang) (˝VLit "*"%string) [˝VVar 0; ˝VVar 3]
+            ]))
+      ]
+    )
+  ] (EApp (˝VFunId (0, 2)) [e; d]) 
+.
+
+Theorem fact_tailrec_eval_ex:
+  forall (z : Z) (z' : Z), (0 <= z)%Z ->
+  exists (y : Z),
+  ⟨ [], (tailrec_fact (˝VLit z) (˝VLit z')) ⟩ -->* RValSeq [VLit y] /\ (y = Z.of_nat (Factorial.fact (Z.to_nat z)) * z')%Z.
+Proof.
+  solve_symbolically z z'.
+  
+  destruct PreCond0. subst.
+  rewrite Z.mul_assoc. f_equal.
+  rewrite <- positive_nat_Z.
+  rewrite <- Nat2Z.inj_mul. f_equal.
+  assert (1%Z = Z.of_nat (Z.to_nat 1%Z))%Z by lia. rewrite H0. clear H0.
+  rewrite <- Nat2Z.inj_sub;[|lia].
+  do 2 rewrite Nat2Z.id.
+  remember (Pos.to_nat p) as k.
+  pose proof Pos2Nat.is_pos p.
+  destruct k; try lia.
+  simpl.
+  rewrite Nat.sub_0_r. lia. 
+Qed.
+
+Definition timestwo (e : Exp) : Exp :=
+  ELetRec [
+      (1, °ECall (˝erlang) (˝VLit "*"%string) [˝VVar 1; ˝VLit 2%Z]
+      
+      )
+    ] (EApp (˝VFunId (0, 1)) [e]).
+
+Definition timestwo' (e : Exp) : Exp :=
+  °ECall (˝erlang) (˝VLit "*"%string) [e; ˝VLit 2%Z].
+
+Theorem timestwo_ex:
+  forall (z : Z), True ->
+  exists (y : Z),
+  ⟨ [], (timestwo (˝VLit z)) ⟩ -->* RValSeq [VLit y] /\ (y = z * 2)%Z.
+Proof.
+  solve_symbolically z.
+Qed.
+
+Theorem timestwo'_ex:
+  forall (z : Z), True ->
+  exists (y : Z),
+  ⟨ [], (timestwo' (˝VLit z)) ⟩ -->* RValSeq [VLit y] /\ (y = z * 2)%Z.
+Proof.
+  solve_symbolically z.
+Qed.
+
+Definition times_two_simple (e : Exp) : Exp :=
+  (EExp (ECall (VVal (VLit (Atom "erlang"%string))) (VVal (VLit (Atom "*"%string))) [e;(VVal (VLit (Integer (2))))])).
+
+Theorem times_two_simple_ex:
+  forall (z : Z), True ->
+  exists (y : Z),
+  ⟨ [], (times_two_simple (˝VLit z)) ⟩ -->* RValSeq [VLit y] /\ (y = z * 2)%Z.
+Proof.
+  solve_symbolically z.
+Qed.
+
+Definition times_two_rec (e : Exp) : Exp := ELetRec [
+(1, (EExp (ECase (VVal (VVar 1)) 
+[
+  ([(PLit (Integer (0)))], (VVal (VLit (Atom "true"%string))), (VVal (VLit (Integer (0)))));
+  ([PVar], (VVal (VLit (Atom "true"%string))), 
+    (EExp (ELet 1 (EExp (ECall (VVal (VLit (Atom "erlang"%string))) (VVal (VLit (Atom "-"%string))) [(VVal (VVar 0));(VVal (VLit (Integer (1))))])) 
+    (EExp (ECall (VVal (VLit (Atom "erlang"%string))) (VVal (VLit (Atom "+"%string))) [(EExp (EApp (VVal (VFunId (2, 1))) [(VVal (VVar 0))]));(VVal (VLit (Integer (2))))])))))])))] 
+
+(EApp (VVal (VFunId (0, 1))) [e]).
+
+Theorem times_two_rec_ex:
+  forall (z : Z), (0 <= z)%Z ->
+  exists (y : Z),
+  ⟨ [], (times_two_rec (˝VLit z)) ⟩ -->* RValSeq [VLit y] /\ (y = z * 2)%Z.
+Proof.
+  solve_symbolically z.
+Qed.
+
+Definition plus_nums_simple (e f : Exp) : Exp :=
+(EExp (ECall (VVal (VLit (Atom "erlang"%string))) (VVal (VLit (Atom "+"%string))) [e;f])).
+
+Theorem plus_nums_simple_ex:
+  forall (z : Z) (z' : Z), True ->
+  exists (y : Z),
+  ⟨ [], (plus_nums_simple (˝VLit z) (˝VLit z')) ⟩ -->* RValSeq [VLit y] /\ (y = z + z')%Z.
+Proof.
+  solve_symbolically z.
+Qed.
+
+Definition plus_nums_rec (e f : Exp) := ELetRec [(2, (EExp (ECase (VVal (VVar 1)) [([(PLit (Integer (0)))], (VVal (VLit (Atom "true"%string))), (VVal (VVar 2)));([PVar], (VVal (VLit (Atom "true"%string))), (EExp (ELet 1 (EExp (ECall (VVal (VLit (Atom "erlang"%string))) (VVal (VLit (Atom "-"%string))) [(VVal (VVar 0));(VVal (VLit (Integer (1))))])) (EExp (ELet 1 (EExp (ECall (VVal (VLit (Atom "erlang"%string))) (VVal (VLit (Atom "+"%string))) [(VVal (VVar 4));(VVal (VLit (Integer (1))))])) (EExp (EApp (VVal (VFunId (3, 2))) [(VVal (VVar 1));(VVal (VVar 0))])))))))])))] (EApp (VVal (VFunId (0, 2))) [e;f]).
+
+Theorem plus_nums_rec_ex:
+  forall (z : Z),
+  exists (y : Z),
+  ⟨ [], (plus_nums_rec (˝VLit z) (˝VLit 0%Z)) ⟩ -->* RValSeq [VLit y] /\ (y = z)%Z.
+Proof.
+  (* This cannot be proven by induction, since the goal is too specific. *)
+Abort.
+
+Theorem plus_nums_rec_ex':
+  forall (z : Z) (z' : Z), (z >= 0)%Z ->
+  exists (y : Z),
+  ⟨ [], (plus_nums_rec (˝VLit z) (˝VLit z')) ⟩ -->* RValSeq [VLit y] /\ (y = z + z')%Z.
+Proof.
+  solve_symbolically z z'.
+Qed.
+
+
+Definition isitzero_atom (e : Exp) : Exp :=
+(EExp (ECase (e) [([(PLit (Integer (0)))], (VVal (VLit (Atom "true"%string))), (VVal (VLit (Atom "true"%string))));([PVar], (VVal (VLit (Atom "true"%string))), (VVal (VLit (Atom "false"%string))))])).
+
+Theorem isitzero_atom_ex:
+  forall (z : Z), (z >= 0)%Z ->
+  exists (y : string),
+  ⟨ [], (isitzero_atom (˝VLit (Z.succ z))) ⟩ -->* RValSeq [VLit y] /\ (y = "false"%string)%Z.
+Proof.
+  solve_symbolically z.
+Qed.
+
+Definition isitzero_num (e : Exp) : Exp :=
+(EExp (ECase (e) [([(PLit (Integer (0)))], (VVal (VLit (Atom "true"%string))), (VVal (VLit (Integer (1)))));([PVar], (VVal (VLit (Atom "true"%string))), (VVal (VLit (Integer (0)))))])).
+
+Theorem isitzero_num_ex:
+  forall (z : Z), True ->
+  exists (y : Z),
+  ⟨ [], (isitzero_num (˝VLit z)) ⟩ -->* RValSeq [VLit y] /\ ((y = 0)%Z \/ (y = 1)%Z).
+Proof.
+  solve_symbolically z.
+Qed.
+
+Definition isitzero_num_app (e : Exp) : Exp :=
+EExp ( EApp ( EFun 1 (EExp (ECase (VVal (VVar 0)) [([(PLit (Integer (0)))], (VVal (VLit (Atom "true"%string))), (VVal (VLit (Integer (1)))));([PVar], (VVal (VLit (Atom "true"%string))), (VVal (VLit (Integer (0)))))]))) [e]).
+
+Theorem isitzero_num_app_ex:
+  forall (z : Z), True ->
+  exists (y : Z),
+  ⟨ [], (isitzero_num_app (˝VLit z)) ⟩ -->* RValSeq [VLit y] /\ ((y = 0)%Z \/ (y = 1)%Z).
+Proof.
+  solve_symbolically z.
+Qed.
+
+Definition isitzero_atom_app (e : Exp) : Exp :=
+EExp ( EApp ( EFun 1(EExp (ECase (VVal (VVar 0)) [([(PLit (Integer (0)))], (VVal (VLit (Atom "true"%string))), (VVal (VLit (Atom "true"%string))));([PVar], (VVal (VLit (Atom "true"%string))), (VVal (VLit (Atom "false"%string))))]))) [e]).
+
+Theorem isitzero_atom_app_ex:
+  forall (z : Z), (z > 0)%Z ->
+  exists (y : string),
+  ⟨ [], (isitzero_atom_app (˝VLit z)) ⟩ -->* RValSeq [VLit y] /\ (y = "false"%string).
+Proof.
+  solve_symbolically z.
+Qed.
+
+Theorem timestwo_ex':
+  forall (z : Z),
+  exists (y : Z),
+  ⟨ [], (times_two_simple (˝VLit z)) ⟩ -->* RValSeq [VLit y] /\ (y = z * 2)%Z.
+Proof.
+  solve_symbolically z.
+Qed.
+
+Definition times_two_simple_app (e : Exp) : Exp :=
+  EExp (EApp (EExp (EFun 1 (EExp (ECall (VVal (VLit (Atom "erlang"%string))) (VVal (VLit (Atom "*"%string))) [(VVal (VVar 0));(VVal (VLit (Integer (2))))])))) [e]).
+
+Theorem timestwo_ex'':
+  forall (z : Z),
+  exists (y : Z),
+  ⟨ [], (times_two_simple_app (˝VLit z)) ⟩ -->* RValSeq [VLit y] /\ (y = z * 2)%Z.
+Proof.
+  solve_symbolically z.
+Qed.
+
+Theorem timestwo_ex''':
+  forall (z : Z), (0 <= z)%Z ->
+  exists (y : Z),
+  ⟨ [], (times_two_rec (˝VLit z)) ⟩ -->* RValSeq [VLit y] /\ (y = z * 2)%Z.
+Proof.
+  solve_symbolically z.
+Qed.
+
+
+
+
+
+
+
+
+
+
+
